Main.lean
@@ -1,15 +1,11 @@
-import LeanSAT.External.Solver
-import LeanSAT.LRAT.LRATChecker
-import LeanSAT.LRAT.LRATCheckerSound
-import LeanSAT.External.LRAT
-import LeanSAT.Reflect.Tactics.SatDecide
+import LeanSAT.Reflect.LRAT
 
-open Dimacs LRAT
+open LRAT
 
 def main : List String → IO Unit := fun args => do
   let prfFile := args[0]!
   let t1 ← IO.monoMsNow
-  let content ← SatDecide.readFileQuick prfFile
+  let content ← BVDecide.readFileQuick prfFile
   let t2 ← IO.monoMsNow
   let some output := parseLRATProof content | throw <| .userError "failed to parse"
   let t3 ← IO.monoMsNow
